Challenge/Modexp/Submission/Proofs/Bytecode/Artifact.lean
@@ -2444,7 +2444,7 @@ def submissionInstructions : List Instr :=
   YulEvmCompiler.Instr.op EvmSemantics.Operation.CALLDATALOAD,
   YulEvmCompiler.Instr.push 1 1,
   YulEvmCompiler.Instr.op EvmSemantics.Operation.MOD,
-  YulEvmCompiler.Instr.op EvmSemantics.Operation.MUL,
+  YulEvmCompiler.Instr.op EvmSemantics.Operation.AND,
   YulEvmCompiler.Instr.push 0 0,
   YulEvmCompiler.Instr.op EvmSemantics.Operation.MSTORE,
   YulEvmCompiler.Instr.push 1 32,
